FTLR - Cas (WIP)

theories/ftlr/Cas.v
@@ -17,12 +17,428 @@ Section fundamental.
   Implicit Types interp : (D).
 
 
+
+
+  (* The necessary resources to close the region again, except for the points to predicate, which we will store separately *)
+  (* Since we will store a new word into a, we do not need to remember its validity *)
+  Definition region_open_resources (a pc_a : Addr) pc_w : iProp Σ :=
+    (▷ interp pc_w ∗ ((▷ ∃ w0, a ↦ₐ w0 ∗ interp w0) ={⊤ ∖ ↑logN.@pc_a ∖ ↑logN.@a,⊤ ∖ ↑logN.@pc_a}=∗ emp))%I.
+
+  Lemma store_inr_eq {regs i r p0 b0 e0 a0 p1 b1 e1 a1}:
+    reg_allows_store i regs r p0 b0 e0 a0 →
+    read_reg_inr regs i r p1 b1 e1 a1 →
+    p0 = p1 ∧ b0 = b1 ∧ e0 = e1 ∧ a0 = a1.
+  Proof.
+      intros Hrar H3.
+      pose (Hrar' := Hrar).
+      destruct Hrar' as (Hinr0 & _). destruct H3 as [Hinr1 | Hinl1].
+      * rewrite Hinr0 in Hinr1. inversion Hinr1.
+        subst;auto.
+      * destruct Hinl1 as [z Hinl1]. rewrite Hinl1 in Hinr0. by exfalso.
+  Qed.
+
+  (* Description of what the resources are supposed to look like after opening the region if we need to, but before closing the region up again*)
+  Definition allow_store_res r1 (regs : Reg) i pc_a a p b e :=
+    (⌜read_reg_inr regs i r1 p b e a⌝ ∗
+      if decide (reg_allows_store i regs r1 p b e a ∧ a ≠ pc_a) then
+          |={⊤ ∖ ↑logN.@pc_a,⊤ ∖ ↑logN.@pc_a ∖ ↑logN.@a}=> ∃ w, a ↦ₐ w ∗ region_open_resources a pc_a w
+    else True)%I.
+
+  Definition allow_store_mem i r1 (regs : Reg) pc_a pc_w (mem : gmap Addr Word) p b e a :=
+    (⌜read_reg_inr regs i r1 p b e a⌝ ∗
+    if decide (reg_allows_store i regs r1 p b e a ∧ a ≠ pc_a) then
+         ∃ w, ⌜mem = <[a:=w]> (<[pc_a:=pc_w]> ∅)⌝ ∗ region_open_resources a pc_a w
+    else ⌜mem = <[pc_a:=pc_w]> ∅⌝)%I.
+
+  (* TODO - we need a new definition of region_open_resources, in particular, we need to remember
+            the validity of the word in the memory *)
+   (* Definition allow_load_mem r (regs : Reg) i (pc_a : Addr) (pc_w : Word) (mem : gmap Addr Word) (a : Addr) p b e := *)
+   (*  (⌜read_reg_inr regs i r p b e a⌝ ∗ *)
+   (*  if decide (reg_allows_store i regs r p b e a ∧ a ≠ pc_a) then *)
+   (*       ∃ w, ⌜mem = <[a:=w]> (<[pc_a:=pc_w]> ∅)⌝ ∗ (region_open_resources a pc_a w) (* ∗ interp w *) *)
+   (*  else  ⌜mem = <[pc_a:=pc_w]> ∅⌝)%I. *)
+
+   (* Lemma allow_store_implies_load_mem i r1 (regs : Reg) pc_a pc_w *)
+   (*   (mem : gmap Addr Word) p b e a : *)
+   (*   allow_store_mem i r1 regs pc_a pc_w mem p b e a *)
+   (*   -∗ allow_load_mem r1 regs i pc_a pc_w mem a p b e. *)
+   (* Proof. *)
+   (*   iIntros "HmemStore". *)
+   (*   rewrite /allow_store_mem /allow_load_mem. *)
+   (*   iFrame *)
+   (*   iDestruct "HmemStore" as "[? HmemStore]" ; iFrame. *)
+
+
+
+  Lemma create_store_res:
+    ∀ (r : leibnizO Reg) (i: CoreN) (p : Perm)
+      (b e a : Addr) (r1 : RegName) (p0 : Perm)
+      (b0 e0 a0 : Addr),
+      read_reg_inr (<[(i, PC):=WCap p b e a]> r) i r1 p0 b0 e0 a0
+      → (∀ (r1 : RegName) v, ⌜r1 ≠ PC⌝ → ⌜r !! (i, r1) = Some v⌝ → (fixpoint interp1) v)
+          -∗ allow_store_res r1 (<[(i, PC):=WCap p b e a]> r) i a a0 p0 b0 e0.
+  Proof.
+    intros r i p b e a r1 p0 b0 e0 a0 HVr1.
+    iIntros "#Hreg".
+    iFrame "%".
+    case_decide as Hallows.
+    - destruct Hallows as ((Hrinr & Hra & Hwb) & Haeq).
+      apply andb_prop in Hwb as [Hle Hge].
+      revert Hle Hge. rewrite !Z.leb_le Z.ltb_lt =>Hle Hge.
+      assert (r1 ≠ PC) as n. refine (addr_ne_reg_ne Hrinr _ Haeq). by rewrite lookup_insert.
+      rewrite lookup_insert_ne in Hrinr; last by congruence.
+      iDestruct ("Hreg" $! r1 _ n Hrinr) as "Hvsrc".
+      iAssert (inv (logN.@a0) ((interp_ref_inv a0) interp))%I as "#Hinva".
+      { iApply (write_allowed_inv with "Hvsrc"); auto. }
+      iFrame "∗ #".
+      iMod (inv_acc with "Hinva") as "[Hinv Hcls']";[solve_ndisj|].
+      iDestruct "Hinv" as (w) "[>Ha0 #Hinv]".
+      iExists w. iFrame. done.
+    - done.
+  Qed.
+
+
+  Lemma store_res_implies_mem_map:
+    ∀ (r : leibnizO Reg) (i: CoreN)
+       (a a0 : Addr) (w : Word) (r1 : RegName) p1 b1 e1,
+      allow_store_res r1 r i a a0 p1 b1 e1
+      -∗ a ↦ₐ w
+      ={⊤ ∖ ↑logN.@a, if decide (reg_allows_store i r r1 p1 b1 e1 a0 ∧ a0 ≠ a) then ⊤ ∖ ↑logN.@a ∖ ↑logN.@a0
+                      else ⊤ ∖ ↑logN.@a}=∗ ∃ mem0 : gmap Addr Word,
+          allow_store_mem i r1 r a w mem0 p1 b1 e1 a0
+            ∗ ▷ ([∗ map] a0↦w ∈ mem0, a0 ↦ₐ w).
+  Proof.
+    intros r i a a0 w r1 p1 b1 e1.
+    iIntros "HStoreRes Ha".
+    iDestruct "HStoreRes" as "(% & HStoreRes)".
+
+    case_decide as Hallows.
+    - iMod "HStoreRes" as (w0) "[Ha0 HStoreRest]".
+      iExists _.
+      iSplitL "HStoreRest".
+      * iFrame "%".
+        case_decide; last by exfalso.
+        iExists w0. iSplitR; auto.
+      * iModIntro. iNext.
+        destruct Hallows as ((Hrinr & Hra & Hwb) & Hne).
+        iApply memMap_resource_2ne; auto; iFrame.
+    - iExists _.
+      iSplitR "Ha".
+      + iFrame "%".
+        case_decide; first by exfalso. auto.
+      + iModIntro. iNext. by iApply memMap_resource_1.
+  Qed.
+
+
+  Lemma mem_map_implies_pure_conds:
+    ∀ (r : leibnizO Reg) (i: CoreN)
+      (a a0 : Addr) (w : Word) (r1 : RegName)
+      (mem0 : gmap Addr Word) p b e,
+        allow_store_mem i r1 r a w mem0 p b e a0
+        -∗ ⌜mem0 !! a = Some w⌝
+          ∗ ⌜allow_store_map_or_true i r1 r mem0⌝.
+  Proof.
+    iIntros (r i a a0 w r1 mem0 p b e) "HStoreMem".
+    iDestruct "HStoreMem" as "(% & HStoreRes)".
+    case_decide as Hallows.
+    - pose(Hallows' := Hallows).
+      destruct Hallows' as ((Hrinr & Hra & Hwb) & Hne).
+      iDestruct "HStoreRes" as (w0 ->) "HStoreRest".
+      iSplitR. rewrite lookup_insert_ne; auto. by rewrite lookup_insert.
+      iExists p,b,e,a0. iSplit;auto.
+      iPureIntro. case_decide;auto.
+      exists w0. by simplify_map_eq.
+    - iDestruct "HStoreRes" as "->".
+      iSplitR. by rewrite lookup_insert.
+      iExists p,b,e,a0. repeat iSplitR; auto.
+      case_decide as Hdec1; last by done.
+      apply not_and_l in Hallows as [Hallows | Hallows]; try contradiction.
+      assert (a0 = a) as ->.
+      { apply finz_to_z_eq, Z.eq_dne. intros Hcontr. apply Hallows. by intros ->. }
+      simplify_map_eq. eauto.
+  Qed.
+
+   Lemma mem_map_recover_res:
+    ∀ (r : leibnizO Reg) (i: CoreN)
+       (a : Addr) (w : Word) (src : RegName) p0
+       (b0 e0 a0 : Addr) (mem0 : gmap Addr Word) storev loadv,
+      reg_allows_store i r src p0 b0 e0 a0
+      → mem0 !! a0 = Some loadv
+      → allow_store_mem i src r a w mem0 p0 b0 e0 a0
+        -∗ ([∗ map] a1↦w ∈ (<[a0:=storev]> mem0), a1 ↦ₐ w)
+        -∗ interp storev
+        ={if decide (reg_allows_store i r src p0 b0 e0 a0 ∧ a0 ≠ a) then ⊤ ∖ ↑logN.@a ∖ ↑logN.@a0 else ⊤ ∖ ↑logN.@a,⊤ ∖ ↑logN.@a}=∗
+            if decide (reg_allows_store i r src p0 b0 e0 a0 ∧ a0 = a) then a ↦ₐ storev else a ↦ₐ w.
+  Proof.
+    intros r i a w src p0 b0 e0 a0 mem0 storev loadv Hrar Hloadv.
+    iIntros "HLoadMem Hmem Hvalid".
+    iDestruct "HLoadMem" as "[% HLoadRes]".
+    (* destruct (load_inr_eq Hrar H0) as (<- & <- &<- &<- &<-). *)
+    case_decide as Hdec. destruct Hdec as [Hallows Heq].
+    -  destruct Hallows as [Hrinr [Hra Hwb] ].
+       iDestruct "HLoadRes" as (w0) "[-> [Hval Hcls] ]".
+       simplify_map_eq. rewrite insert_insert.
+       rewrite memMap_resource_2ne; last auto. iDestruct "Hmem" as  "[Ha1 Haw]".
+       iMod ("Hcls" with "[Ha1 Hvalid]") as "_";[iNext;iExists storev;iFrame|]. iModIntro.
+       rewrite decide_False; [done|]. apply not_and_r. right. auto.
+    - apply not_and_r in Hdec as [| <-%dec_stable].
+      * by exfalso.
+      * iDestruct "HLoadRes" as "->".
+        rewrite insert_insert.
+        rewrite -memMap_resource_1. simplify_map_eq. by iFrame.
+  Qed.
+
+
+  (*  Lemma mem_map_recover_res_neq: *)
+  (*   ∀ (r : leibnizO Reg) (i: CoreN) *)
+  (*      (a : Addr) (w : Word) (src : RegName) p0 *)
+  (*      (b0 e0 a0 : Addr) (mem0 : gmap Addr Word) loadv, *)
+  (*     reg_allows_store i r src p0 b0 e0 a0 *)
+  (*     → mem0 !! a0 = Some loadv *)
+  (*     → allow_store_mem i src r a w mem0 p0 b0 e0 a0 *)
+  (*       -∗ ([∗ map] a1↦w ∈ mem0, a1 ↦ₐ w) *)
+  (*       ={if decide (reg_allows_store i r src p0 b0 e0 a0 ∧ a0 ≠ a) then *)
+  (*           ⊤ ∖ ↑logN.@a ∖ ↑logN.@a0 else ⊤ ∖ ↑logN.@a,⊤ ∖ ↑logN.@a}=∗ a ↦ₐ w. *)
+  (*           (* if decide (reg_allows_store i r src p0 b0 e0 a0 ∧ a0 = a) then a ↦ₐ storev else . *) *)
+  (* Proof. *)
+  (*   intros r i a w src p0 b0 e0 a0 mem0 loadv Hrar Hloadv. *)
+  (*   iIntros "HLoadMem Hmem". *)
+  (*   iDestruct "HLoadMem" as "[% HLoadRes]". *)
+  (*   (* destruct (load_inr_eq Hrar H0) as (<- & <- &<- &<- &<-). *) *)
+  (*   case_decide as Hdec. destruct Hdec as [Hallows Heq]. *)
+  (*   -  destruct Hallows as [Hrinr [Hra Hwb] ]. *)
+  (*      iDestruct "HLoadRes" as (w0) "[-> [Hval Hcls] ]". *)
+  (*      simplify_map_eq. *)
+  (*      rewrite memMap_resource_2ne; last auto. iDestruct "Hmem" as  "[Ha1 Haw]". *)
+  (*      iMod ("Hcls" with "[Ha1]") as "_";[iNext;iExists loadv;iFrame|]. iModIntro. *)
+  (*      rewrite decide_False; [done|]. apply not_and_r. right. auto. *)
+  (*   - apply not_and_r in Hdec as [| <-%dec_stable]. *)
+  (*     * by exfalso. *)
+  (*     * iDestruct "HLoadRes" as "->". *)
+  (*       rewrite insert_insert. *)
+  (*       rewrite -memMap_resource_1. simplify_map_eq. by iFrame. *)
+  (* Qed. *)
+
   Lemma cas_case (r : leibnizO Reg) (p : Perm) (b e a : Addr) (w : Word)
     (loc cond newvalue: RegName) (i: CoreN) P :
     ftlr_instr r p b e a w (CAS loc cond newvalue) i P.
   Proof.
     intros Hp Hsome i' Hbae Hi.
     iIntros "#IH #Hinv #Hinva #Hreg #[Hread Hwrite] Ha HP Hcls HPC Hmap".
-  Admitted.
 
+
+    rewrite delete_insert_delete.
+    iDestruct ((big_sepM_delete _ _ (i, PC)) with "[HPC Hmap]") as "Hmap /=";
+      [apply lookup_insert|rewrite delete_insert_delete;iFrame|]. simpl.
+
+    (* To read out PC's name later, and needed when calling wp_load *)
+    assert(∀ x : RegName, is_Some (<[(i, PC):=WCap p b e a]> r !! (i, x))) as Hsome'.
+    {
+      intros. destruct (decide (x = PC)).
+      rewrite e0 lookup_insert; unfold is_Some. by eexists.
+        by rewrite lookup_insert_ne ; simplify_pair_eq.
+    }
+
+    (* Initializing the names for the values of Hsrc now, to instantiate the existentials in step 1 *)
+    assert (∃ p0 b0 e0 a0 , read_reg_inr (<[(i,PC):=WCap p b e a]> r) i loc p0 b0 e0 a0) as [p0 [b0 [e0 [a0 HVloc] ] ] ].
+    {
+      specialize Hsome' with loc as Hloc.
+      destruct Hloc as [wloc Hsomeloc].
+      unfold read_reg_inr. destruct wloc. all: repeat eexists.
+      right. by exists z. by left.
+    }
+
+     assert (∃ oldv, (<[(i, PC):=WCap p b e a]> r) !! (i, newvalue) = Some oldv) as [oldv Hwoa].
+    { specialize Hsome' with newvalue as Hnewvalue.
+      destruct Hnewvalue as [wnewv Hsomenewvalue].
+      exists wnewv. by rewrite Hsomenewvalue.
+    }
+
+    (* Step 1: open the region, if necessary, and store all the resources obtained from the region in allow_load_res *)
+    iDestruct (create_store_res with "Hreg") as "HStoreRes"; eauto.
+
+    (* Step2: derive the concrete map of memory we need, and any spatial predicates holding over it *)
+    iMod (store_res_implies_mem_map with "HStoreRes Ha") as (mem) "[HStoreMem >HMemRes]".
+
+    (* Step 3:  derive the non-spatial conditions over the memory map*)
+    iDestruct (mem_map_implies_pure_conds with "HStoreMem") as %(HReadPC & HStoreAP); auto.
+
+    iApply (wp_Cas with "[Hmap HMemRes]"); eauto.
+    { by rewrite lookup_insert. }
+    { rewrite /regs_of_core /subseteq /map_subseteq /set_subseteq_instance. intros rr ?.
+      apply elem_of_gmap_dom. set_solver. }
+    { iSplitR "Hmap"; auto. }
+    iNext. iIntros (regs' mem' retv). iDestruct 1 as (HSpec) "[Hmem Hmap]".
+
+    iDestruct ("Hread" with "HP") as "#Hw".
+
+    destruct HSpec as [ * -> -> Hfail | * ? ? ? ? -> Hincr|* ? ? ? -> ? ? Hincr].
+    - (* Failure *)
+      rewrite /allow_store_res /allow_store_mem.
+      destruct (decide (reg_allows_store i regs' loc p0 b0 e0 a0 ∧ a0 ≠ a)).
+      + iDestruct "HStoreMem" as "(%&H)".
+        iDestruct "H" as (w') "(->&[Hres Hcls'])". rewrite /region_open_resources.
+        destruct a1. simplify_map_eq. rewrite memMap_resource_2ne; last auto.
+        iDestruct "Hmem" as "[Ha0 Ha]".
+        iMod ("Hcls'" with "[Ha0 Hres]");[iExists w';iFrame|iModIntro].
+        iMod ("Hcls" with "[Ha HP]");[iExists w;iFrame|iModIntro].
+        iApply wp_pure_step_later; auto.
+        iApply wp_value; auto.
+      + iModIntro. iDestruct "HStoreMem" as "(_&->)". rewrite -memMap_resource_1.
+        iMod ("Hcls" with "[Hmem HP]");[iExists w;iFrame|iModIntro].
+        iApply wp_pure_step_later; auto.
+        iApply wp_value; auto.
+
+    - (* Success - Equality  *)
+      apply incrementPC_Some_inv in Hincr.
+      destruct Hincr as (?&?&?&?&?&?&?&?).
+      iApply wp_pure_step_later; auto.
+      specialize (store_inr_eq H0 HVloc) as (-> & -> & -> & ->).
+
+    {  (* The stored value is valid *)
+      iAssert (interp newv) as "#Hvalidnewv".
+      { destruct (<[(i, PC):=WCap p b e a]> r !! (i, newvalue)) eqn:Hsomenewvalue
+         ;simplify_map_eq by simplify_pair_eq.
+        destruct (decide (newvalue = PC)).
+        - subst. simplify_map_eq by simplify_pair_eq. iFrame "Hinv".
+        - simplify_map_eq by simplify_pair_eq. iSpecialize ("Hreg" $! i _ _ n Hsomenewvalue).
+          iFrame "Hreg".
+      }
+
+      (* Step 4: return all the resources we had in order to close the second location in the region, in the cases where we need to *)
+      iMod (mem_map_recover_res with "HStoreMem Hmem Hvalidnewv") as "Ha";[eauto|eauto|iModIntro].
+
+      iMod ("Hcls" with "[HP Ha]").
+      { simplify_map_eq.
+        case_decide as Hwrite.
+        - case_decide.
+          + iNext. iExists oldv.
+            iDestruct ("Hwrite" with "Hvalidnewv") as "HPstore".
+            iFrame "∗ #".
+          + iNext. iExists w. iFrame.
+        - rewrite decide_False. iNext. iExists w. iFrame.
+          intros [Hcontr ->].
+          apply Hwrite. exists loc.
+          destruct Hcontr as (Hlookup & Hwa & Hwb). simplify_map_eq.
+          apply andb_prop in Hwb.
+          revert Hwb. rewrite Z.leb_le Z.ltb_lt. intros. eexists _.
+          split_and!; done.
+      }
+
+      simplify_map_eq  by simplify_pair_eq.
+      (* rewrite insert_insert. *)
+
+      iApply ("IH" with "[%] [] Hmap");auto.
+      { intros; cbn.
+        destruct (decide ( cond = x4 )) ; subst.
+        simplify_map_eq ; by eexists.
+        rewrite lookup_insert_ne ; simplify_map_eq by simplify_pair_eq.
+        destruct (decide ( PC = x4 )) ; subst.
+        simplify_map_eq ; by eexists.
+        rewrite lookup_insert_ne ; simplify_map_eq by simplify_pair_eq.
+        by apply Hsome. }
+      { iIntros (j ri v Hri Hvs).
+        destruct (decide ((j, ri) = (i, cond))).
+        { simplify_pair_eq.
+          rewrite lookup_insert in Hvs; auto. inversion Hvs.
+          destruct (decide (a = a0)).
+          - simplify_eq. iFrame "Hw".
+          - simplify_eq. rewrite lookup_insert_ne in H4
+            ; simplify_map_eq by simplify_pair_eq.
+            iApply "Hreg"; eauto.
+        }
+        rewrite lookup_insert_ne in Hvs ; simplify_map_eq by simplify_pair_eq.
+        iApply "Hreg" ; eauto.
+        simplify_pair_eq.
+        apply pair_neq_inv' ; by apply not_eq_sym.
+      }
+      { destruct ( decide (cond = PC))
+        ; subst
+        ; [|rewrite lookup_insert_ne in H4]
+        ; simplify_map_eq by simplify_pair_eq
+        ; do 3 iModIntro
+        ; iApply interp_cap_range ; eauto
+        ; destruct Hp ; subst ; auto.
+      }
+    }
+
+    - (* Success - Non Equality  *)
+      apply incrementPC_Some_inv in Hincr.
+      destruct Hincr as (?&?&?&?&?&?&?&?).
+      iApply wp_pure_step_later; auto.
+      specialize (store_inr_eq H0 HVloc) as (-> & -> & -> & ->).
+
+
+    {  (* The stored value is valid *)
+      iAssert (interp newv) as "#Hvalidnewv".
+      { destruct (<[(i, PC):=WCap p b e a]> r !! (i, newvalue)) eqn:Hsomenewvalue
+         ;simplify_map_eq by simplify_pair_eq.
+        destruct (decide (newvalue = PC)).
+        - subst. simplify_map_eq by simplify_pair_eq. iFrame "Hinv".
+        - simplify_map_eq by simplify_pair_eq. iSpecialize ("Hreg" $! i _ _ n Hsomenewvalue).
+          iFrame "Hreg".
+      }
+
+      (* Step 4: return all the resources we had in order to close the second location in the region, in the cases where we need to *)
+      iMod (mem_map_recover_res with "[HStoreMem] [Hmem] [Hvalidnewv]") as "Ha"
+      ; try eauto.
+      { admit. (* modify the definition of the lemma and don't store the new value *) }
+      iModIntro.
+
+      iMod ("Hcls" with "[HP Ha]").
+      { simplify_map_eq.
+        case_decide as Hwrite.
+        - case_decide.
+          + iNext. iExists oldv.
+            iDestruct ("Hwrite" with "Hvalidnewv") as "HPstore".
+            iFrame "∗ #".
+          + iNext. iExists w. iFrame.
+        - rewrite decide_False. iNext. iExists w. iFrame.
+          intros [Hcontr ->].
+          apply Hwrite. exists loc.
+          destruct Hcontr as (Hlookup & Hwa & Hwb). simplify_map_eq.
+          apply andb_prop in Hwb.
+          revert Hwb. rewrite Z.leb_le Z.ltb_lt. intros. eexists _.
+          split_and!; done.
+      }
+
+      simplify_map_eq  by simplify_pair_eq.
+      (* rewrite insert_insert. *)
+
+      iApply ("IH" with "[%] [] Hmap");auto.
+      { intros; cbn.
+        destruct (decide ( cond = x4 )) ; subst.
+        simplify_map_eq ; by eexists.
+        rewrite lookup_insert_ne ; simplify_map_eq by simplify_pair_eq.
+        destruct (decide ( PC = x4 )) ; subst.
+        simplify_map_eq ; by eexists.
+        rewrite lookup_insert_ne ; simplify_map_eq by simplify_pair_eq.
+        by apply Hsome. }
+      { iIntros (j ri v Hri Hvs).
+        destruct (decide ((j, ri) = (i, cond))).
+        { simplify_pair_eq.
+          rewrite lookup_insert in Hvs; auto. inversion Hvs.
+          destruct (decide (a = a0)).
+          - simplify_eq. iFrame "Hw".
+          - simplify_eq. rewrite lookup_insert_ne in H5
+            ; simplify_map_eq by simplify_pair_eq.
+            admit.
+        }
+        rewrite lookup_insert_ne in Hvs ; simplify_map_eq by simplify_pair_eq.
+        iApply "Hreg" ; eauto.
+        simplify_pair_eq.
+        apply pair_neq_inv' ; by apply not_eq_sym.
+      }
+      { destruct ( decide (cond = PC))
+        ; subst
+        ; [|rewrite lookup_insert_ne in H5]
+        ; simplify_map_eq by simplify_pair_eq
+        ; do 3 iModIntro.
+        admit.
+        iApply interp_cap_range ; eauto
+        ; destruct Hp ; subst ; auto.
+      }
+    }
+    Unshelve. all: auto.
+  Admitted.
 End fundamental.
